src/Lib/Lib.v
@@ -37,3 +37,12 @@ Definition int_of_bool (b : bool) := Int.repr (if b then 255 else 0).
 Definition bool_of_int (i : int) := 
   if (i == 0)%int then false else true.
 
+(* Find composite *)
+Fixpoint find_cs (id : ident) cs : option composite_definition :=
+  match cs with
+  | Composite i s_u m a :: css => if (i =? id)%positive
+                             then Some (Composite i s_u m a)
+                             else find_cs id css
+  | [] => None
+  end.
+
