src/Lib/VstLib.v
@@ -1,6 +1,6 @@
 Require Import Core.Core.
 Require Import VST.floyd.proofauto.
-Require Import Clight.asn_codecs_prim.
+Require Import Clight.asn_codecs_prim Clight.asn_application.
 Require Import Lib.
 
 Require Export Lib.
@@ -22,3 +22,7 @@ Definition asn_dec_rval_s := Tstruct _asn_dec_rval_s noattr.
 Definition mk_dec_rval code consumed := 
   (Vint (Int.repr code), Vint (Int.repr consumed)).
 
+(* Overrun callback key *)
+Definition enc_key_s := Tstruct _overrun_encoder_key noattr.
+Definition mk_enc_key (buf : val) size comp_size := 
+  (buf, (Vint (Int.repr size), Vint (Int.repr comp_size))). 
